ver3_less_complex/common/seq.dfy
@@ -1,0 +1,16 @@
+
+
+module M_Seq {
+    import opened Std.Collections.Seq
+
+    lemma Lemma_PrefixOfTwoPrefixSeqAlsoPrefix<T>(pre1 : seq<T>,
+                                            pre2 : seq<T>,
+                                            seq1 : seq<T>,
+                                            seq2 : seq<T>)
+    requires pre1 <= seq1
+    requires pre2 <= seq2
+    requires seq1 <= seq2 || seq2 <= seq1
+    ensures pre1 <= pre2 || pre2 <= pre1
+    {
+    }
+}
